$$ \frac{n!}{(n-k)!} $$

$$ \binom{n}{k} = \frac{n!}{k!(n-k)!} $$

$$ n^{k} $$

$$ \binom{n+k-1}{k} = \frac{(n+k-1)!}{k!(n-1)!} $$ 

$$ H = -\frac{1}{\ln K} \cdot \sum_{j=1}^{k} \left( h_j \cdot \ln h_j \right) $$ 

$$ \text{AD}_x = \frac{\sum_i^n \left| x_i - \bar{x}\right|}{n} $$ 

$$ s_x^2 = \frac{\sum_i^n \left( x_i - \bar{x}\right)^2}{n} $$ 

$$ s_x = \sqrt{s_x^2} = \sqrt{\frac{\sum_i^n \left( x_i - \bar{x}\right)^2}{n}}  $$ 

$$ \hat{\sigma}_x^2 = \frac{\sum_i^n \left( x_i - \bar{x}\right)^2}{n-1} $$ 

$$ \hat{\sigma}_x = \sqrt{\hat{\sigma}_x^2} = \sqrt{\frac{\sum_i^n \left( x_i - \bar{x}\right)^2}{n-1}} $$ 

$$ SE = \frac{s_x}{\sqrt{n}} $$ 

$$ F = \frac{\sigma^2_1}{\sigma^2_2} $$ 

$$ F = \frac{MSS_\text{zw}}{MSS_\text{inn}} $$ 

$$ t = \frac{\bar{x} - \mu_0}{\hat{\sigma}_{\bar{x}}} $$ 

$$ z = \sqrt{n} \left(\frac{\bar{x}-\mu_0}{\sigma}\right) $$ 

$$ z = \left(\frac{\bar{x}-\mu_0}{SE}\right) $$ 

$$ \chi^2 = \sum_\text{Zellen} \frac{(\text{Beo} - \text{Modell})^2}{\text{Modell}} $$ 

$$ \chi^2_\text{Yates} = \sum_\text{Zellen} \frac{( |\text{Beo} - \text{Modell}| - 0.5)^2}{\text{Modell}} $$ 

$$ L_{\chi^2} = 2 \sum \text{Beo} \ln \left( \frac{\text{Beo}}{\text{Modell}} \right) $$ 

$$ P(A|B) = \frac{P(B | A)\, P(A)}{P(B)} $$ 

$$ P(H_{0}|E) = \frac{P(E | H_{0})\, P(H_{0})}{P(E)} $$ 
